Remvoe Avl from ContractSem so that this file can be replaced with a translation from Lem

ContractSem.thy
@@ -5,7 +5,7 @@ suitable for formal verification of a single account.  *}
 
 theory ContractSem
 
-imports Main "~~/src/HOL/Word/Word" "~~/src/HOL/Data_Structures/AVL_Map" "./ContractEnv" "./Instructions" "./KEC"
+imports Main "~~/src/HOL/Word/Word" "./ContractEnv" "./Instructions" "./KEC"
 
 begin
 
@@ -140,7 +140,7 @@ text "For performance reasons, the instructions are stored in an AVL tree that a
 looking up instructions from the program counters."
 
 record program = 
-  program_content :: "(int \<times> inst) avl_tree"
+  program_content :: "int \<Rightarrow> inst option"
   -- {* a binary search tree that allows looking up instructions from positions *}
   program_length  :: int -- {* the length of the program in bytes *}
   program_annotation :: "int \<Rightarrow> annotation list"
@@ -151,80 +151,13 @@ text {* The empty program is easy to define. *}
 abbreviation empty_program :: program
 where
 "empty_program \<equiv>
-  \<lparr> program_content = \<langle>\<rangle>
+  \<lparr> program_content = (\<lambda> _. None)
   , program_length = 0
   , program_annotation = (\<lambda> _. []) \<rparr>"
 
 
 subsection "Translating an Instruction List into a Program"
 
-subsubsection {* Integers can be compared *}
-
-text {* The AVL library requires the keys to be comparable.  We represent program positions 
-by integers.  So we have to prove that integers belong to the type class \textit{cmp} with the
-usual comparison operators.  *}
-
-instantiation int :: cmp
-begin
-definition cmp_int :: "int \<Rightarrow> int \<Rightarrow> Cmp.cmp"
-where
-cmp_int_def : " cmp_int x y =
-  (if x < y then Cmp.LT else (if x = y then Cmp.EQ else Cmp.GT))"
-
-instance proof
- fix x y :: int show "(cmp x y = cmp.LT) = (x < y)"
-  apply(simp add: cmp_int_def)
-  done
- fix x y :: int show "(cmp x y = cmp.EQ) = (x = y)"
-  apply(simp add: cmp_int_def)
-  done
- fix x y :: int show "(cmp x y = cmp.GT) = (x > y)"
-  apply(simp add: cmp_int_def)
-  done
-qed
-
-end
-
-subsubsection {* Storing the immediate values in the AVL tree *}
-
-text {* The data region of PUSH\_N instructions are encoded as
- Unknown instructions.  Here is a utility function that
- inserts a byte sequence after a specified index in the AVL tree. *}
-
-fun store_byte_list_in_program ::
-  "int (* initial position in the AVL *) \<Rightarrow> byte list (* the data *) \<Rightarrow>
-   (int * inst) avl_tree (* original AVL *)  \<Rightarrow>
-   (int * inst) avl_tree (* result *)"
-where
-  "store_byte_list_in_program _ [] orig = orig"
-| "store_byte_list_in_program pos (h # t) orig =
-     store_byte_list_in_program (pos + 1) t (update pos (Unknown h) orig)"
-declare store_byte_list_in_program.simps [simp]
-
-subsubsection {* Storing a program in the AVL tree *}
-
-text {* Here is a function that stores a list of instructions in the AVL tree.
-The initial key is specified.  The following keys are computed using the sizes
-of instructions being inserted.
-*}
-
-fun program_content_of_lst ::
-  "int (* initial position in the AVL *) \<Rightarrow> inst list (* instructions *)
-   \<Rightarrow> (int * inst) avl_tree (* result *)"
-where
-  "program_content_of_lst _ [] = Leaf"
-  -- {* the empty program is translated into the empty tree. *}
-| "program_content_of_lst pos (Stack (PUSH_N bytes) # rest) =
-   store_byte_list_in_program (pos + 1) bytes 
-   (update pos (Stack (PUSH_N bytes))
-          (program_content_of_lst (pos + 1 + (int (length bytes))) rest))"
-  -- {* The PUSH instruction is translated together with the immediate value. *}
-| "program_content_of_lst pos (Annotation _ # rest) =
-    program_content_of_lst pos rest"
-  -- {* Annotations are skipped because they do not belong in this AVL tree. *}
-| "program_content_of_lst pos (i # rest) =
-   update pos i (program_content_of_lst (pos + 1) rest)"
-  -- {* The other instructions are simply inserted into the AVL tree. *}
 
 subsubsection {* Storing annotations in a program in a mapping *}
 
@@ -254,11 +187,14 @@ declare program_annotation_of_lst.simps [simp]
 subsubsection {* Translating a list of instructions into a program *}
 
 text {* The results of the above translations are packed together in a record. *}
+text {* For efficiency reasons, the program content is going to be packed as
+an AVL tree, but this particular encoding is not part of the Lem definition.
+So such encoders are parametrised here.*}
 
-abbreviation program_of_lst :: "inst list \<Rightarrow> program"
+abbreviation program_of_lst :: "inst list \<Rightarrow> (inst list \<Rightarrow> (int \<Rightarrow> inst option)) \<Rightarrow> program"
 where
-"program_of_lst lst \<equiv>
-  \<lparr> program_content = program_content_of_lst 0 lst
+"program_of_lst lst program_content_formatter \<equiv>
+  \<lparr> program_content = program_content_formatter lst
   , program_length = int (length lst)
   , program_annotation = program_annotation_of_lst 0 lst
   \<rparr>"
@@ -271,7 +207,7 @@ text {* Such a memory is here implemented by a lookup on an AVL tree.*}
 abbreviation program_as_memory :: "program \<Rightarrow> memory"
 where
 "program_as_memory p idx \<equiv>
-   (case lookup (program_content p) (uint idx) of
+   (case (program_content p) (uint idx) of
      None \<Rightarrow> 0
    | Some inst \<Rightarrow> inst_code inst ! 0)"
    
@@ -408,7 +344,7 @@ text {* Peeking the next instruction: *}
 abbreviation venv_next_instruction :: "variable_env \<Rightarrow> constant_env \<Rightarrow> inst option"
 where
 "venv_next_instruction v c \<equiv>
-   lookup (program_content (cenv_program c)) (venv_pc v)"
+   (program_content (cenv_program c)) (venv_pc v)"
    
 text {* Advancing the program counter: *}
 abbreviation venv_advance_pc :: "constant_env \<Rightarrow> variable_env \<Rightarrow> variable_env"
@@ -1336,7 +1272,7 @@ inductive build_venv_returned ::
 "account_state \<Rightarrow> return_result \<Rightarrow> variable_env \<Rightarrow> bool"
 where
 venv_returned:
-"  is_call_like (lookup (program_content a_code) (v_pc - 1)) \<Longrightarrow>
+"  is_call_like ((program_content a_code) (v_pc - 1)) \<Longrightarrow>
    new_bal \<ge> a_bal \<Longrightarrow> (* the balance might have increased *)
    build_venv_returned
 
@@ -1397,7 +1333,7 @@ where
       [] \<Rightarrow> None
    | (recovered, _, _) # _ \<Rightarrow>
       (if is_call_like (* check the previous instruction *)
-        (lookup (program_content (account_code a))
+        (program_content (account_code a)
          (venv_pc recovered - 1)) then
        Some (recovered
          \<lparr>venv_stack := 0 (* indicating failure *) # venv_stack recovered\<rparr>)
@@ -1493,132 +1429,6 @@ declare word_rcat_def [simp]
         unat_def [simp]
         bin_rcat_def [simp]
         
-text {* I do not allow the AVL library to perform updates at arbitrary moments,
-because that causes exponentially expensive computation (as measured with
-the number of elements *) *}
-declare update.simps [simp del]
-declare lookup.simps [simp del]
-
-text {* Instead, I only allow the following operations to happen (from left to right). *}
-
-lemma updateL [simp] : "update x y Leaf = Node 1 Leaf (x,y) Leaf"
-apply(simp add: update.simps)
-done
-
-lemma updateN_EQ [simp]: "cmp x a = EQ \<Longrightarrow> update x y (Node h l (a, b) r) = Node h l (x, y) r"
-apply(simp add: update.simps)
-done
-
-lemma updateN_GT [simp]: "cmp x a = GT \<Longrightarrow> update x y (Node h l (a, b) r) = balR l (a, b) (update x y r)"
-apply(simp add: update.simps)
-done
-
-lemma updateN_LT [simp]: "cmp x a = LT \<Longrightarrow> update x y (Node h l (a, b) r) = balL (update x y l) (a, b) r"
-apply(simp add: update.simps)
-done
-
-lemma lookupN_EQ [simp]: "cmp x a = EQ \<Longrightarrow> lookup (Node h l (a, b) r) x = Some b"
-apply(simp add: lookup.simps)
-done
-
-lemma lookupN_GT [simp]: "cmp x a = GT \<Longrightarrow> lookup (Node h l (a, b) r) x = lookup r x"
-apply(simp add: lookup.simps)
-done
-
-lemma lookupN_LT [simp]: "cmp x a = LT \<Longrightarrow> lookup (Node h l (a, b) r) x = lookup l x"
-apply(simp add: lookup.simps)
-done
-
-lemma lookupL [simp]: "lookup Leaf x = None"
-apply(simp add: lookup.simps)
-done
-
-lemma nodeLL [simp] : "node Leaf a Leaf == Node 1 Leaf a Leaf"
-apply(simp add:node_def)
-done
-
-lemma nodeLN [simp] : "node Leaf a (Node rsize rl rv rr) == Node (rsize + 1) Leaf a (Node rsize rl rv rr)"
-apply(simp add:node_def)
-done
-
-lemma nodeNL [simp] : "node \<langle>lsize, ll, lv, lr\<rangle> a \<langle>\<rangle> == Node (lsize + 1) (Node lsize ll lv lr) a Leaf"
-apply(simp add: node_def)
-done
-
-lemma nodeNN [simp] : "node (Node lsize ll lv lr) a (Node rsize rl rv rr) == Node (max lsize rsize + 1) (Node lsize ll lv lr) a (Node rsize rl rv rr)"
-apply(simp add: node_def)
-done
-
-lemma balL_neq_NL [simp]:
-  "lh \<noteq> Suc (Suc 0) \<Longrightarrow>
-   balL (Node lh ll b lr) a Leaf = node (Node lh ll b lr) a Leaf"
-apply(simp add: balL_def)
-done
-
-lemma balL_neq_Lr [simp]:
-  "balL Leaf a r = node Leaf a r"
-apply(simp add: balL_def)
-done
-
-lemma balL_neq_NN [simp]:
-  "lh \<noteq> Suc (Suc rh) \<Longrightarrow>
-   balL (Node lh ll lx lr) a (Node rh rl rx rr) = node (Node lh ll lx lr) a (Node rh rl rx rr)"
-apply(simp add: balL_def)
-done
-
-lemma balL_eq_heavy_r_rL [simp]:
-  "ht bl < ch \<Longrightarrow>
-   balL (Node (Suc (Suc 0)) bl b (Node ch cl c cr)) a Leaf = node (node bl b cl) c (node cr a Leaf)
-   "
-apply(simp add: balL_def)
-done
-
-lemma balL_eq_heavy_r_rN [simp]:
-  "hl = Suc (Suc rh) \<Longrightarrow>
-   ht bl < ch \<Longrightarrow>
-   balL (Node hl bl b (Node ch cl c cr)) a (Node rh rl rx rr) = node (node bl b cl) c (node cr a (Node rh rl rx rr))
-   "
-apply(simp add: balL_def)
-done
-
-lemma balL_eq_heavy_l [simp]:
-  "hl = ht r + 2 \<Longrightarrow>
-   ht bl \<ge> ht br \<Longrightarrow>
-   balL (Node hl bl b br) a r = node bl b (node br a r)"
-apply(simp add: balL_def)
-done
-
-lemma balR_neq_xL [simp]:
-  "balR l a Leaf = node l a Leaf"
-apply(simp add: balR_def)
-done
-
-lemma balR_neq_LN [simp]:
-  "rh \<noteq> Suc (Suc 0) \<Longrightarrow>
-   balR Leaf a (Node rh rl rx rr) = node Leaf a (Node rh rl rx rr)"
-apply(simp add: balR_def)
-done
-
-lemma balR_neq_NN [simp]:
-  "rh \<noteq> Suc (Suc lh) \<Longrightarrow>
-   balR (Node lh ll lx lr) a (Node rh rl rx rr) = node (Node lh ll lx lr) a (Node rh rl rx rr)"
-apply(simp add: balR_def)
-done
-
-lemma balR_eq_heavy_l [simp]:
-  "bh = ht l + 2 \<Longrightarrow>
-   ch > ht br \<Longrightarrow>
-   balR l a (Node bh (Node ch cl c cr) b br) =
-   node (node l a cl) c (node cr b br)"
-apply(simp add: balR_def)
-done
-
-lemma balR_eq_heavy_r [simp]:
-  "bh = ht l + 2 \<Longrightarrow>
-   ht bl \<le> ht br \<Longrightarrow>
-   balR l a (Node bh bl b br) = node (node l a bl) b br"
-apply(simp add: balR_def)
-done
 
 
 text {* There is a common pattern for checking a predicate. *}
