ProgramInAvl.thy
@@ -1,0 +1,209 @@
+theory ProgramInAvl
+
+imports Main "./Instructions"  "~~/src/HOL/Data_Structures/AVL_Map"
+
+begin
+
+subsubsection {* Integers can be compared *}
+
+text {* The AVL library requires the keys to be comparable.  We represent program positions 
+by integers.  So we have to prove that integers belong to the type class \textit{cmp} with the
+usual comparison operators.  *}
+
+instantiation int :: cmp
+begin
+definition cmp_int :: "int \<Rightarrow> int \<Rightarrow> Cmp.cmp"
+where
+cmp_int_def : " cmp_int x y =
+  (if x < y then Cmp.LT else (if x = y then Cmp.EQ else Cmp.GT))"
+
+declare cmp_int_def [simp]
+  
+instance proof
+ fix x y :: int show "(cmp x y = cmp.LT) = (x < y)"
+  apply(simp add: cmp_int_def)
+  done
+ fix x y :: int show "(cmp x y = cmp.EQ) = (x = y)"
+  apply(simp add: cmp_int_def)
+  done
+ fix x y :: int show "(cmp x y = cmp.GT) = (x > y)"
+  apply(simp add: cmp_int_def)
+  done
+qed
+
+end
+
+subsubsection {* Storing the immediate values in the AVL tree *}
+
+text {* The data region of PUSH\_N instructions are encoded as
+ Unknown instructions.  Here is a utility function that
+ inserts a byte sequence after a specified index in the AVL tree. *}
+
+fun store_byte_list_in_program ::
+  "int (* initial position in the AVL *) \<Rightarrow> byte list (* the data *) \<Rightarrow>
+   (int * inst) avl_tree (* original AVL *)  \<Rightarrow>
+   (int * inst) avl_tree (* result *)"
+where
+  "store_byte_list_in_program _ [] orig = orig"
+| "store_byte_list_in_program pos (h # t) orig =
+     store_byte_list_in_program (pos + 1) t (update pos (Unknown h) orig)"
+declare store_byte_list_in_program.simps [simp]
+
+subsubsection {* Storing a program in the AVL tree *}
+
+text {* Here is a function that stores a list of instructions in the AVL tree.
+The initial key is specified.  The following keys are computed using the sizes
+of instructions being inserted.
+*}
+
+fun program_avl_of_lst ::
+  "int (* initial position in the AVL *) \<Rightarrow> inst list (* instructions *)
+   \<Rightarrow> (int * inst) avl_tree (* result *)"
+where
+  "program_avl_of_lst _ [] = Leaf"
+  -- {* the empty program is translated into the empty tree. *}
+| "program_avl_of_lst pos (Stack (PUSH_N bytes) # rest) =
+   store_byte_list_in_program (pos + 1) bytes 
+   (update pos (Stack (PUSH_N bytes))
+          (program_avl_of_lst (pos + 1 + (int (length bytes))) rest))"
+  -- {* The PUSH instruction is translated together with the immediate value. *}
+| "program_avl_of_lst pos (Annotation _ # rest) =
+    program_avl_of_lst pos rest"
+  -- {* Annotations are skipped because they do not belong in this AVL tree. *}
+| "program_avl_of_lst pos (i # rest) =
+   update pos i (program_avl_of_lst (pos + 1) rest)"
+  -- {* The other instructions are simply inserted into the AVL tree. *}
+  
+abbreviation program_content_of_lst :: "inst list \<Rightarrow> (int \<Rightarrow> inst option)"
+where
+"program_content_of_lst lst \<equiv>
+   (lookup (program_avl_of_lst 0 lst))"
+
+text {* I do not allow the AVL library to perform updates at arbitrary moments,
+because that causes exponentially expensive computation (as measured with
+the number of elements *) *}
+declare update.simps [simp del]
+declare lookup.simps [simp del]
+
+text {* Instead, I only allow the following operations to happen (from left to right). *}
+
+lemma updateL [simp] : "update x y Leaf = Node 1 Leaf (x,y) Leaf"
+apply(simp add: update.simps)
+done
+
+lemma updateN_EQ [simp]: "cmp x a = EQ \<Longrightarrow> update x y (Node h l (a, b) r) = Node h l (x, y) r"
+apply(simp add: update.simps)
+done
+
+lemma updateN_GT [simp]: "cmp x a = GT \<Longrightarrow> update x y (Node h l (a, b) r) = balR l (a, b) (update x y r)"
+apply(simp add: update.simps)
+done
+
+lemma updateN_LT [simp]: "cmp x a = LT \<Longrightarrow> update x y (Node h l (a, b) r) = balL (update x y l) (a, b) r"
+apply(simp add: update.simps)
+done
+
+lemma lookupN_EQ [simp]: "cmp x a = EQ \<Longrightarrow> lookup (Node h l (a, b) r) x = Some b"
+apply(simp add: lookup.simps)
+done
+
+lemma lookupN_GT [simp]: "cmp x a = GT \<Longrightarrow> lookup (Node h l (a, b) r) x = lookup r x"
+apply(simp add: lookup.simps)
+done
+
+lemma lookupN_LT [simp]: "cmp x a = LT \<Longrightarrow> lookup (Node h l (a, b) r) x = lookup l x"
+apply(simp add: lookup.simps)
+done
+
+lemma lookupL [simp]: "lookup Leaf x = None"
+apply(simp add: lookup.simps)
+done
+
+lemma nodeLL [simp] : "node Leaf a Leaf == Node 1 Leaf a Leaf"
+apply(simp add:node_def)
+done
+
+lemma nodeLN [simp] : "node Leaf a (Node rsize rl rv rr) == Node (rsize + 1) Leaf a (Node rsize rl rv rr)"
+apply(simp add:node_def)
+done
+
+lemma nodeNL [simp] : "node \<langle>lsize, ll, lv, lr\<rangle> a \<langle>\<rangle> == Node (lsize + 1) (Node lsize ll lv lr) a Leaf"
+apply(simp add: node_def)
+done
+
+lemma nodeNN [simp] : "node (Node lsize ll lv lr) a (Node rsize rl rv rr) == Node (max lsize rsize + 1) (Node lsize ll lv lr) a (Node rsize rl rv rr)"
+apply(simp add: node_def)
+done
+
+lemma balL_neq_NL [simp]:
+  "lh \<noteq> Suc (Suc 0) \<Longrightarrow>
+   balL (Node lh ll b lr) a Leaf = node (Node lh ll b lr) a Leaf"
+apply(simp add: balL_def)
+done
+
+lemma balL_neq_Lr [simp]:
+  "balL Leaf a r = node Leaf a r"
+apply(simp add: balL_def)
+done
+
+lemma balL_neq_NN [simp]:
+  "lh \<noteq> Suc (Suc rh) \<Longrightarrow>
+   balL (Node lh ll lx lr) a (Node rh rl rx rr) = node (Node lh ll lx lr) a (Node rh rl rx rr)"
+apply(simp add: balL_def)
+done
+
+lemma balL_eq_heavy_r_rL [simp]:
+  "ht bl < ch \<Longrightarrow>
+   balL (Node (Suc (Suc 0)) bl b (Node ch cl c cr)) a Leaf = node (node bl b cl) c (node cr a Leaf)
+   "
+apply(simp add: balL_def)
+done
+
+lemma balL_eq_heavy_r_rN [simp]:
+  "hl = Suc (Suc rh) \<Longrightarrow>
+   ht bl < ch \<Longrightarrow>
+   balL (Node hl bl b (Node ch cl c cr)) a (Node rh rl rx rr) = node (node bl b cl) c (node cr a (Node rh rl rx rr))
+   "
+apply(simp add: balL_def)
+done
+
+lemma balL_eq_heavy_l [simp]:
+  "hl = ht r + 2 \<Longrightarrow>
+   ht bl \<ge> ht br \<Longrightarrow>
+   balL (Node hl bl b br) a r = node bl b (node br a r)"
+apply(simp add: balL_def)
+done
+
+lemma balR_neq_xL [simp]:
+  "balR l a Leaf = node l a Leaf"
+apply(simp add: balR_def)
+done
+
+lemma balR_neq_LN [simp]:
+  "rh \<noteq> Suc (Suc 0) \<Longrightarrow>
+   balR Leaf a (Node rh rl rx rr) = node Leaf a (Node rh rl rx rr)"
+apply(simp add: balR_def)
+done
+
+lemma balR_neq_NN [simp]:
+  "rh \<noteq> Suc (Suc lh) \<Longrightarrow>
+   balR (Node lh ll lx lr) a (Node rh rl rx rr) = node (Node lh ll lx lr) a (Node rh rl rx rr)"
+apply(simp add: balR_def)
+done
+
+lemma balR_eq_heavy_l [simp]:
+  "bh = ht l + 2 \<Longrightarrow>
+   ch > ht br \<Longrightarrow>
+   balR l a (Node bh (Node ch cl c cr) b br) =
+   node (node l a cl) c (node cr b br)"
+apply(simp add: balR_def)
+done
+
+lemma balR_eq_heavy_r [simp]:
+  "bh = ht l + 2 \<Longrightarrow>
+   ht bl \<le> ht br \<Longrightarrow>
+   balR l a (Node bh bl b br) = node (node l a bl) b br"
+apply(simp add: balR_def)
+done
+
+end
